examples/demo.v
@@ -356,9 +356,9 @@ Inductive T : Type :=
 Quote Recursively Definition TT := T.
 
 Unset Strict Unquote Universe Mode.
-Make Definition t := (tSort (NEL.sing (Level.Level "Top.20000", false))).
+Make Definition t := (tSort (Universe.make (Level.Level "Top.20000"))).
 Make Definition t' := (tSort fresh_universe).
-Make Definition myProp := (tSort (Universe.make' (Level.lProp, false))).
+Make Definition myProp := (tSort (Universe.make Level.lProp)).
 Make Definition myProp' := (tSort Universe.type0m).
 Make Definition mySet := (tSort (Universe.make Level.lSet)).
 
